Add std/record2 and std/record3.

theories/std/record3.v
@@ -1,6 +1,6 @@
 From ml Require Import
   prelude.
-From ml.lang Require Import
+From ml.language Require Import
   notations
   proofmode.
 From ml.std Require Export
@@ -8,41 +8,42 @@ From ml.std Require Export
 
 Section heapGS.
   Context `{!heapGS Σ}.
+
   Implicit Types l : loc.
 
   Definition record3_make : val :=
     λ: "v₀" "v₁" "v₂",
       let: "l" := AllocN #3 "v₀" in
-      "l".(1) <- "v₁" ;;
-      "l".(2) <- "v₂" ;;
+      "l".[1] <- "v₁" ;;
+      "l".[2] <- "v₂" ;;
       "l".
 
   Definition record3_model l dq v₀ v₁ v₂ : iProp Σ :=
-    l.(0) ↦{dq} v₀ ∗
-    l.(1) ↦{dq} v₁ ∗
-    l.(2) ↦{dq} v₂.
+    l.[0] ↦{dq} v₀ ∗
+    l.[1] ↦{dq} v₁ ∗
+    l.[2] ↦{dq} v₂.
 
   Lemma record3_model_eq l dq v₀ v₁ v₂ :
     record3_model l dq v₀ v₁ v₂ ⊣⊢
-    l.(0) ↦{dq} v₀ ∗ l.(1) ↦{dq} v₁ ∗ l.(2) ↦{dq} v₂.
+    l.[0] ↦{dq} v₀ ∗ l.[1] ↦{dq} v₁ ∗ l.[2] ↦{dq} v₂.
   Proof.
-    done.
+    iSmash.
   Qed.
   Lemma record3_model_eq_1 l dq v₀ v₁ v₂ :
-    record3_model l dq v₀ v₁ v₂ -∗
-      l.(0) ↦{dq} v₀ ∗
-      l.(1) ↦{dq} v₁ ∗
-      l.(2) ↦{dq} v₂.
+    record3_model l dq v₀ v₁ v₂ ⊢
+      l.[0] ↦{dq} v₀ ∗
+      l.[1] ↦{dq} v₁ ∗
+      l.[2] ↦{dq} v₂.
   Proof.
-    done.
+    iSmash.
   Qed.
   Lemma record3_model_eq_2 l dq v₀ v₁ v₂ :
-    l.(0) ↦{dq} v₀ -∗
-    l.(1) ↦{dq} v₁ -∗
-    l.(2) ↦{dq} v₂ -∗
+    l.[0] ↦{dq} v₀ -∗
+    l.[1] ↦{dq} v₁ -∗
+    l.[2] ↦{dq} v₂ -∗
     record3_model l dq v₀ v₁ v₂.
   Proof.
-    rewrite /record3_model. auto with iFrame.
+    iSmash.
   Qed.
 
   #[global] Instance record3_model_timeless l dq v₀ v₁ v₂ :
@@ -68,7 +69,7 @@ Section heapGS.
   Qed.
 
   Lemma record3_model_valid l dq v₀ v₁ v₂ :
-    record3_model l dq v₀ v₁ v₂ -∗
+    record3_model l dq v₀ v₁ v₂ ⊢
     ⌜✓ dq⌝.
   Proof.
     iIntros "(Hv₀ & Hv₁ & Hv₂)". iApply (mapsto_valid with "Hv₀").
@@ -83,7 +84,7 @@ Section heapGS.
     iDestruct (mapsto_combine with "Hv₀1 Hv₀2") as "(Hv₀ & <-)".
     iDestruct (mapsto_combine with "Hv₁1 Hv₁2") as "(Hv₁ & <-)".
     iDestruct (mapsto_combine with "Hv₂1 Hv₂2") as "(Hv₂ & <-)".
-    iSplit; last done. iFrame.
+    iSmash.
   Qed.
   Lemma record3_model_valid_2 l dq1 v₀1 v₁1 v₂1 dq2 v₀2 v₁2 v₂2 :
     record3_model l dq1 v₀1 v₁1 v₂1 -∗
@@ -93,15 +94,14 @@ Section heapGS.
     iIntros "Hl1 Hl2".
     iDestruct (record3_model_combine with "Hl1 Hl2") as "(Hl & %)".
     iDestruct (record3_model_valid with "Hl") as %?.
-    done.
+    iSmash+.
   Qed.
   Lemma record3_model_agree l dq1 v₀1 v₁1 v₂1 dq2 v₀2 v₁2 v₂2 :
     record3_model l dq1 v₀1 v₁1 v₂1 -∗
     record3_model l dq2 v₀2 v₁2 v₂2 -∗
     ⌜v₀1 = v₀2 ∧ v₁1 = v₁2 ∧ v₂1 = v₂2⌝.
   Proof.
-    iIntros "Hl1 Hl2".
-    iDestruct (record3_model_valid_2 with "Hl1 Hl2") as %?. naive_solver.
+    iSmash.
   Qed.
   Lemma record3_model_dfrac_ne l1 dq1 v₀1 v₁1 v₂1 l2 dq2 v₀2 v₁2 v₂2 :
     ¬ ✓ (dq1 ⋅ dq2) →
@@ -110,118 +110,132 @@ Section heapGS.
     ⌜l1 ≠ l2⌝.
   Proof.
     iIntros "% Hl1 Hl2" (->).
-    iDestruct (record3_model_valid_2 with "Hl1 Hl2") as %?. naive_solver.
+    iDestruct (record3_model_valid_2 with "Hl1 Hl2") as %?.
+    naive_solver.
   Qed.
   Lemma record3_model_ne l1 v₀1 v₁1 v₂1 l2 dq2 v₀2 v₁2 v₂2 :
     record3_model l1 (DfracOwn 1) v₀1 v₁1 v₂1 -∗
     record3_model l2 dq2 v₀2 v₁2 v₂2 -∗
     ⌜l1 ≠ l2⌝.
   Proof.
-    iApply record3_model_dfrac_ne. intros []%exclusive_l. apply _.
+    iSmash.
   Qed.
   Lemma record3_model_exclusive l v₀1 v₁1 v₂1 v₀2 v₁2 v₂2 :
     record3_model l (DfracOwn 1) v₀1 v₁1 v₂1 -∗
     record3_model l (DfracOwn 1) v₀2 v₁2 v₂2 -∗
     False.
   Proof.
-    iIntros "Hl1 Hl2".
-    iDestruct (record3_model_ne with "Hl1 Hl2") as %?. naive_solver.
+    iSmash.
   Qed.
   Lemma record3_model_persist l dq v₀ v₁ v₂ :
-    record3_model l dq v₀ v₁ v₂ ==∗
+    record3_model l dq v₀ v₁ v₂ ⊢ |==>
     record3_model l DfracDiscarded v₀ v₁ v₂.
   Proof.
-    iIntros "(Hv₀ & Hv₁ & Hv₂)".
-    iMod (mapsto_persist with "Hv₀") as "$".
-    iMod (mapsto_persist with "Hv₁") as "$".
-    iMod (mapsto_persist with "Hv₂") as "$".
-    done.
+    iSmash.
   Qed.
 
   Lemma record3_dfrac_relax dq l v₀ v₁ v₂ :
     ✓ dq →
-    record3_model l (DfracOwn 1) v₀ v₁ v₂ ==∗
+    record3_model l (DfracOwn 1) v₀ v₁ v₂ ⊢ |==>
     record3_model l dq v₀ v₁ v₂.
   Proof.
     iIntros "% (Hv₀ & Hv₁ & Hv₂)".
     iMod (mapsto_dfrac_relax with "Hv₀") as "Hv₀"; first done.
     iMod (mapsto_dfrac_relax with "Hv₁") as "Hv₁"; first done.
     iMod (mapsto_dfrac_relax with "Hv₂") as "Hv₂"; first done.
-    iFrame. done.
+    iSmash.
   Qed.
 
   Lemma record3_make_spec v₀ v₁ v₂ :
     {{{ True }}}
       record3_make v₀ v₁ v₂
-    {{{ l, RET #l; record3_model l (DfracOwn 1) v₀ v₁ v₂ ∗ meta_token l ⊤ }}}.
+    {{{ l,
+      RET #l;
+      record3_model l (DfracOwn 1) v₀ v₁ v₂ ∗
+      meta_token l ⊤
+    }}}.
   Proof.
     iIntros "%Φ _ HΦ".
     wp_rec. wp_pures.
-    wp_apply (wp_allocN with "[//]"); first done. iIntros "%l (Hl & Hmeta & _)". rewrite loc_add_0.
+    wp_apply (wp_allocN with "[//]"); first done. iIntros "%l (Hl & Hmeta & _)". rewrite Loc.add_0.
     wp_pures.
     iDestruct (array_cons with "Hl") as "(Hv₀ & Hl)".
-    iEval (setoid_rewrite <- loc_add_0) in "Hv₀".
-    iDestruct (array_cons with "Hl") as "(Hv₁ & Hl)".
-    iDestruct (array_singleton with "Hl") as "Hv₂".
-    rewrite loc_add_assoc Z.add_1_r -Z.two_succ.
-    wp_store. wp_store.
-    iApply "HΦ". iFrame. done.
+    iEval (setoid_rewrite <- Loc.add_0) in "Hv₀".
+    iSmash.
   Qed.
 
   Lemma record3_get0_spec l dq v₀ v₁ v₂ :
-    {{{ record3_model l dq v₀ v₁ v₂ }}}
-      !#l.(0)
-    {{{ RET v₀; record3_model l dq v₀ v₁ v₂ }}}.
+    {{{
+      record3_model l dq v₀ v₁ v₂
+    }}}
+      !#l.[0]
+    {{{
+      RET v₀;
+      record3_model l dq v₀ v₁ v₂
+    }}}.
   Proof.
-    iIntros "%Φ (Hv₀ & Hv₁ & Hv₂) HΦ".
-    wp_load.
-    iApply ("HΦ" with "[$Hv₀ $Hv₁ $Hv₂]").
+    iSmash.
   Qed.
   Lemma record3_get1_spec l dq v₀ v₁ v₂ :
-    {{{ record3_model l dq v₀ v₁ v₂ }}}
-      !#l.(1)
-    {{{ RET v₁; record3_model l dq v₀ v₁ v₂ }}}.
+    {{{
+      record3_model l dq v₀ v₁ v₂
+    }}}
+      !#l.[1]
+    {{{
+      RET v₁;
+      record3_model l dq v₀ v₁ v₂
+    }}}.
   Proof.
-    iIntros "%Φ (Hv₀ & Hv₁ & Hv₂) HΦ".
-    wp_load.
-    iApply ("HΦ" with "[$Hv₀ $Hv₁ $Hv₂]").
+    iSmash.
   Qed.
   Lemma record3_get2_spec l dq v₀ v₁ v₂ :
-    {{{ record3_model l dq v₀ v₁ v₂ }}}
-      !#l.(2)
-    {{{ RET v₂; record3_model l dq v₀ v₁ v₂ }}}.
+    {{{
+      record3_model l dq v₀ v₁ v₂
+    }}}
+      !#l.[2]
+    {{{
+      RET v₂;
+      record3_model l dq v₀ v₁ v₂
+    }}}.
   Proof.
-    iIntros "%Φ (Hv₀ & Hv₁ & Hv₂) HΦ".
-    wp_load.
-    iApply ("HΦ" with "[$Hv₀ $Hv₁ $Hv₂]").
+    iSmash.
   Qed.
 
   Lemma record3_set0_spec l v₀ v₁ v₂ v :
-    {{{ record3_model l (DfracOwn 1) v₀ v₁ v₂ }}}
-      #l.(0) <- v
-    {{{ RET #(); record3_model l (DfracOwn 1) v v₁ v₂ }}}.
+    {{{
+      record3_model l (DfracOwn 1) v₀ v₁ v₂
+    }}}
+      #l.[0] <- v
+    {{{
+      RET #();
+      record3_model l (DfracOwn 1) v v₁ v₂
+    }}}.
   Proof.
-    iIntros "%Φ (Hv₀ & Hv₁ & Hv₂) HΦ".
-    wp_store.
-    iApply ("HΦ" with "[$Hv₀ $Hv₁ $Hv₂]").
+    iSmash.
   Qed.
   Lemma record3_set1_spec l v₀ v₁ v₂ v :
-    {{{ record3_model l (DfracOwn 1) v₀ v₁ v₂ }}}
-      #l.(1) <- v
-    {{{ RET #(); record3_model l (DfracOwn 1) v₀ v v₂ }}}.
+    {{{
+      record3_model l (DfracOwn 1) v₀ v₁ v₂
+    }}}
+      #l.[1] <- v
+    {{{
+      RET #();
+      record3_model l (DfracOwn 1) v₀ v v₂
+    }}}.
   Proof.
-    iIntros "%Φ (Hv₀ & Hv₁ & Hv₂) HΦ".
-    wp_store.
-    iApply ("HΦ" with "[$Hv₀ $Hv₁ $Hv₂]").
+    iSmash.
   Qed.
   Lemma record3_set2_spec l v₀ v₁ v₂ v :
-    {{{ record3_model l (DfracOwn 1) v₀ v₁ v₂ }}}
-      #l.(2) <- v
-    {{{ RET #(); record3_model l (DfracOwn 1) v₀ v₁ v }}}.
+    {{{
+      record3_model l (DfracOwn 1) v₀ v₁ v₂
+    }}}
+      #l.[2] <- v
+    {{{
+      RET #();
+      record3_model l (DfracOwn 1) v₀ v₁ v
+    }}}.
   Proof.
-    iIntros "%Φ (Hv₀ & Hv₁ & Hv₂) HΦ".
-    wp_store.
-    iApply ("HΦ" with "[$Hv₀ $Hv₁ $Hv₂]").
+    iSmash.
   Qed.
 End heapGS.
 
