theories/std/record4.v
@@ -1,6 +1,6 @@
 From ml Require Import
   prelude.
-From ml.lang Require Import
+From ml.language Require Import
   notations
   proofmode.
 From ml.std Require Export
@@ -8,45 +8,46 @@ From ml.std Require Export
 
 Section heapGS.
   Context `{!heapGS Σ}.
+
   Implicit Types l : loc.
 
   Definition record4_make : val :=
     λ: "v₀" "v₁" "v₂" "v₃",
       let: "l" := AllocN #4 "v₀" in
-      "l".(1) <- "v₁" ;;
-      "l".(2) <- "v₂" ;;
-      "l".(3) <- "v₃" ;;
+      "l".[1] <- "v₁" ;;
+      "l".[2] <- "v₂" ;;
+      "l".[3] <- "v₃" ;;
       "l".
 
   Definition record4_model l dq v₀ v₁ v₂ v₃ : iProp Σ :=
-    l.(0) ↦{dq} v₀ ∗
-    l.(1) ↦{dq} v₁ ∗
-    l.(2) ↦{dq} v₂ ∗
-    l.(3) ↦{dq} v₃.
+    l.[0] ↦{dq} v₀ ∗
+    l.[1] ↦{dq} v₁ ∗
+    l.[2] ↦{dq} v₂ ∗
+    l.[3] ↦{dq} v₃.
 
   Lemma record4_model_eq l dq v₀ v₁ v₂ v₃ :
     record4_model l dq v₀ v₁ v₂ v₃ ⊣⊢
-    l.(0) ↦{dq} v₀ ∗ l.(1) ↦{dq} v₁ ∗ l.(2) ↦{dq} v₂ ∗ l.(3) ↦{dq} v₃.
+    l.[0] ↦{dq} v₀ ∗ l.[1] ↦{dq} v₁ ∗ l.[2] ↦{dq} v₂ ∗ l.[3] ↦{dq} v₃.
   Proof.
-    done.
+    iSmash.
   Qed.
   Lemma record4_model_eq_1 l dq v₀ v₁ v₂ v₃ :
-    record4_model l dq v₀ v₁ v₂ v₃ -∗
-      l.(0) ↦{dq} v₀ ∗
-      l.(1) ↦{dq} v₁ ∗
-      l.(2) ↦{dq} v₂ ∗
-      l.(3) ↦{dq} v₃.
+    record4_model l dq v₀ v₁ v₂ v₃ ⊢
+      l.[0] ↦{dq} v₀ ∗
+      l.[1] ↦{dq} v₁ ∗
+      l.[2] ↦{dq} v₂ ∗
+      l.[3] ↦{dq} v₃.
   Proof.
-    done.
+    iSmash.
   Qed.
   Lemma record4_model_eq_2 l dq v₀ v₁ v₂ v₃ :
-    l.(0) ↦{dq} v₀ -∗
-    l.(1) ↦{dq} v₁ -∗
-    l.(2) ↦{dq} v₂ -∗
-    l.(3) ↦{dq} v₃ -∗
+    l.[0] ↦{dq} v₀ -∗
+    l.[1] ↦{dq} v₁ -∗
+    l.[2] ↦{dq} v₂ -∗
+    l.[3] ↦{dq} v₃ -∗
     record4_model l dq v₀ v₁ v₂ v₃.
   Proof.
-   rewrite /record4_model. auto with iFrame.
+    iSmash.
   Qed.
 
   #[global] Instance record4_model_timeless l dq v₀ v₁ v₂ v₃ :
@@ -72,7 +73,7 @@ Section heapGS.
   Qed.
 
   Lemma record4_model_valid l dq v₀ v₁ v₂ v₃ :
-    record4_model l dq v₀ v₁ v₂ v₃ -∗
+    record4_model l dq v₀ v₁ v₂ v₃ ⊢
     ⌜✓ dq⌝.
   Proof.
     iIntros "(Hv₀ & Hv₁ & Hv₂ & Hv₃)". iApply (mapsto_valid with "Hv₀").
@@ -88,7 +89,7 @@ Section heapGS.
     iDestruct (mapsto_combine with "Hv₁1 Hv₁2") as "(Hv₁ & <-)".
     iDestruct (mapsto_combine with "Hv₂1 Hv₂2") as "(Hv₂ & <-)".
     iDestruct (mapsto_combine with "Hv₃1 Hv₃2") as "(Hv₃ & <-)".
-    iSplit; last done. iFrame.
+    iSmash.
   Qed.
   Lemma record4_model_valid_2 l dq1 v₀1 v₁1 v₂1 v₃1 dq2 v₀2 v₁2 v₂2 v₃2 :
     record4_model l dq1 v₀1 v₁1 v₂1 v₃1 -∗
@@ -98,15 +99,14 @@ Section heapGS.
     iIntros "Hl1 Hl2".
     iDestruct (record4_model_combine with "Hl1 Hl2") as "(Hl & %)".
     iDestruct (record4_model_valid with "Hl") as %?.
-    done.
+    iSmash+.
   Qed.
   Lemma record4_model_agree l dq1 v₀1 v₁1 v₂1 v₃1 dq2 v₀2 v₁2 v₂2 v₃2 :
     record4_model l dq1 v₀1 v₁1 v₂1 v₃1 -∗
     record4_model l dq2 v₀2 v₁2 v₂2 v₃2 -∗
     ⌜v₀1 = v₀2 ∧ v₁1 = v₁2 ∧ v₂1 = v₂2 ∧ v₃1 = v₃2⌝.
   Proof.
-    iIntros "Hl1 Hl2".
-    iDestruct (record4_model_valid_2 with "Hl1 Hl2") as %?. naive_solver.
+    iSmash.
   Qed.
   Lemma record4_model_dfrac_ne l1 dq1 v₀1 v₁1 v₂1 v₃1 l2 dq2 v₀2 v₁2 v₂2 v₃2 :
     ¬ ✓ (dq1 ⋅ dq2) →
@@ -115,38 +115,33 @@ Section heapGS.
     ⌜l1 ≠ l2⌝.
   Proof.
     iIntros "% Hl1 Hl2" (->).
-    iDestruct (record4_model_valid_2 with "Hl1 Hl2") as %?. naive_solver.
+    iDestruct (record4_model_valid_2 with "Hl1 Hl2") as %?.
+    naive_solver.
   Qed.
   Lemma record4_model_ne l1 v₀1 v₁1 v₂1 v₃1 l2 dq2 v₀2 v₁2 v₂2 v₃2 :
     record4_model l1 (DfracOwn 1) v₀1 v₁1 v₂1 v₃1 -∗
     record4_model l2 dq2 v₀2 v₁2 v₂2 v₃2 -∗
     ⌜l1 ≠ l2⌝.
   Proof.
-    iApply record4_model_dfrac_ne. intros []%exclusive_l. apply _.
+    iSmash.
   Qed.
   Lemma record4_model_exclusive l v₀1 v₁1 v₂1 v₃1 v₀2 v₁2 v₂2 v₃2 :
     record4_model l (DfracOwn 1) v₀1 v₁1 v₂1 v₃1 -∗
     record4_model l (DfracOwn 1) v₀2 v₁2 v₂2 v₃2 -∗
     False.
   Proof.
-    iIntros "Hl1 Hl2".
-    iDestruct (record4_model_ne with "Hl1 Hl2") as %?. naive_solver.
+    iSmash.
   Qed.
   Lemma record4_model_persist l dq v₀ v₁ v₂ v₃ :
-    record4_model l dq v₀ v₁ v₂ v₃ ==∗
+    record4_model l dq v₀ v₁ v₂ v₃ ⊢ |==>
     record4_model l DfracDiscarded v₀ v₁ v₂ v₃.
   Proof.
-    iIntros "(Hv₀ & Hv₁ & Hv₂ & Hv₃)".
-    iMod (mapsto_persist with "Hv₀") as "$".
-    iMod (mapsto_persist with "Hv₁") as "$".
-    iMod (mapsto_persist with "Hv₂") as "$".
-    iMod (mapsto_persist with "Hv₃") as "$".
-    done.
+    iSmash.
   Qed.
 
   Lemma record4_dfrac_relax dq l v₀ v₁ v₂ v₃ :
     ✓ dq →
-    record4_model l (DfracOwn 1) v₀ v₁ v₂ v₃ ==∗
+    record4_model l (DfracOwn 1) v₀ v₁ v₂ v₃ ⊢ |==>
     record4_model l dq v₀ v₁ v₂ v₃.
   Proof.
     iIntros "% (Hv₀ & Hv₁ & Hv₂ & Hv₃)".
@@ -154,92 +149,111 @@ Section heapGS.
     iMod (mapsto_dfrac_relax with "Hv₁") as "Hv₁"; first done.
     iMod (mapsto_dfrac_relax with "Hv₂") as "Hv₂"; first done.
     iMod (mapsto_dfrac_relax with "Hv₃") as "Hv₃"; first done.
-    iFrame. done.
+    iSmash.
   Qed.
 
   Lemma record4_make_spec v₀ v₁ v₂ v₃ :
     {{{ True }}}
       record4_make v₀ v₁ v₂ v₃
-    {{{ l, RET #l; record4_model l (DfracOwn 1) v₀ v₁ v₂ v₃ ∗ meta_token l ⊤ }}}.
+    {{{ l,
+      RET #l;
+      record4_model l (DfracOwn 1) v₀ v₁ v₂ v₃ ∗
+      meta_token l ⊤
+    }}}.
   Proof.
     iIntros "%Φ _ HΦ".
     wp_rec. wp_pures.
-    wp_apply (wp_allocN with "[//]"); first done. iIntros "%l (Hl & Hmeta & _)". rewrite loc_add_0.
+    wp_apply (wp_allocN with "[//]"); first done. iIntros "%l (Hl & Hmeta & _)". rewrite Loc.add_0.
     wp_pures.
     iDestruct (array_cons with "Hl") as "(Hv₀ & Hl)".
-    iEval (setoid_rewrite <- loc_add_0) in "Hv₀".
-    iDestruct (array_cons with "Hl") as "(Hv₁ & Hl)".
-    iDestruct (array_cons with "Hl") as "(Hv₂ & Hl)".
-    rewrite loc_add_assoc Z.add_1_r -Z.two_succ.
-    iDestruct (array_singleton with "Hl") as "Hv₃".
-    rewrite loc_add_assoc Z.add_1_r. assert (Z.succ 2 = 3)%Z as -> by lia.
-    wp_store. wp_store. wp_store.
-    iApply "HΦ". iFrame. done.
+    iEval (setoid_rewrite <- Loc.add_0) in "Hv₀".
+    iSmash.
   Qed.
 
   Lemma record4_get0_spec l dq v₀ v₁ v₂ v₃ :
-    {{{ record4_model l dq v₀ v₁ v₂ v₃ }}}
-      !#l.(0)
-    {{{ RET v₀; record4_model l dq v₀ v₁ v₂ v₃ }}}.
+    {{{
+      record4_model l dq v₀ v₁ v₂ v₃
+    }}}
+      !#l.[0]
+    {{{
+      RET v₀;
+      record4_model l dq v₀ v₁ v₂ v₃
+    }}}.
   Proof.
-    iIntros "%Φ (Hv₀ & Hv₁ & Hv₂ & Hv₃) HΦ".
-    wp_load.
-    iApply ("HΦ" with "[$Hv₀ $Hv₁ $Hv₂ $Hv₃]").
+    iSmash.
   Qed.
   Lemma record4_get1_spec l dq v₀ v₁ v₂ v₃ :
-    {{{ record4_model l dq v₀ v₁ v₂ v₃ }}}
-      !#l.(1)
-    {{{ RET v₁; record4_model l dq v₀ v₁ v₂ v₃ }}}.
+    {{{
+      record4_model l dq v₀ v₁ v₂ v₃
+    }}}
+      !#l.[1]
+    {{{
+      RET v₁;
+      record4_model l dq v₀ v₁ v₂ v₃
+    }}}.
   Proof.
-    iIntros "%Φ (Hv₀ & Hv₁ & Hv₂ & Hv₃) HΦ".
-    wp_load.
-    iApply ("HΦ" with "[$Hv₀ $Hv₁ $Hv₂ $Hv₃]").
+    iSmash.
   Qed.
   Lemma record4_get2_spec l dq v₀ v₁ v₂ v₃ :
-    {{{ record4_model l dq v₀ v₁ v₂ v₃ }}}
-      !#l.(2)
-    {{{ RET v₂; record4_model l dq v₀ v₁ v₂ v₃ }}}.
+    {{{
+      record4_model l dq v₀ v₁ v₂ v₃
+    }}}
+      !#l.[2]
+    {{{
+      RET v₂;
+      record4_model l dq v₀ v₁ v₂ v₃
+    }}}.
   Proof.
-    iIntros "%Φ (Hv₀ & Hv₁ & Hv₂ & Hv₃) HΦ".
-    wp_load.
-    iApply ("HΦ" with "[$Hv₀ $Hv₁ $Hv₂ $Hv₃]").
+    iSmash.
   Qed.
   Lemma record4_get3_spec l dq v₀ v₁ v₂ v₃ :
-    {{{ record4_model l dq v₀ v₁ v₂ v₃ }}}
-      !#l.(3)
-    {{{ RET v₃; record4_model l dq v₀ v₁ v₂ v₃ }}}.
+    {{{
+      record4_model l dq v₀ v₁ v₂ v₃
+    }}}
+      !#l.[3]
+    {{{
+      RET v₃;
+      record4_model l dq v₀ v₁ v₂ v₃
+    }}}.
   Proof.
-    iIntros "%Φ (Hv₀ & Hv₁ & Hv₂ & Hv₃) HΦ".
-    wp_load.
-    iApply ("HΦ" with "[$Hv₀ $Hv₁ $Hv₂ $Hv₃]").
+    iSmash.
   Qed.
 
   Lemma record4_set0_spec l v₀ v₁ v₂ v₃ v :
-    {{{ record4_model l (DfracOwn 1) v₀ v₁ v₂ v₃ }}}
-      #l.(0) <- v
-    {{{ RET #(); record4_model l (DfracOwn 1) v v₁ v₂ v₃ }}}.
+    {{{
+      record4_model l (DfracOwn 1) v₀ v₁ v₂ v₃
+    }}}
+      #l.[0] <- v
+    {{{
+      RET #();
+      record4_model l (DfracOwn 1) v v₁ v₂ v₃
+    }}}.
   Proof.
-    iIntros "%Φ (Hv₀ & Hv₁ & Hv₂ & Hv₃) HΦ".
-    wp_store.
-    iApply ("HΦ" with "[$Hv₀ $Hv₁ $Hv₂ $Hv₃]").
+    iSmash.
   Qed.
   Lemma record4_set1_spec l v₀ v₁ v₂ v₃ v :
-    {{{ record4_model l (DfracOwn 1) v₀ v₁ v₂ v₃ }}}
-      #l.(1) <- v
-    {{{ RET #(); record4_model l (DfracOwn 1) v₀ v v₂ v₃ }}}.
+    {{{
+      record4_model l (DfracOwn 1) v₀ v₁ v₂ v₃
+    }}}
+      #l.[1] <- v
+    {{{
+      RET #();
+      record4_model l (DfracOwn 1) v₀ v v₂ v₃
+    }}}.
   Proof.
-    iIntros "%Φ (Hv₀ & Hv₁ & Hv₂ & Hv₃) HΦ".
-    wp_store.
-    iApply ("HΦ" with "[$Hv₀ $Hv₁ $Hv₂ $Hv₃]").
+    iSmash.
   Qed.
   Lemma record4_set2_spec l v₀ v₁ v₂ v₃ v :
-    {{{ record4_model l (DfracOwn 1) v₀ v₁ v₂ v₃ }}}
-      #l.(2) <- v
-    {{{ RET #(); record4_model l (DfracOwn 1) v₀ v₁ v v₃ }}}.
+    {{{
+      record4_model l (DfracOwn 1) v₀ v₁ v₂ v₃
+    }}}
+      #l.[2] <- v
+    {{{
+      RET #();
+      record4_model l (DfracOwn 1) v₀ v₁ v v₃
+    }}}.
   Proof.
-    iIntros "%Φ (Hv₀ & Hv₁ & Hv₂ & Hv₃) HΦ".
-    wp_store.
-    iApply ("HΦ" with "[$Hv₀ $Hv₁ $Hv₂ $Hv₃]").
+    iSmash.
   Qed.
 End heapGS.
 
